Unfinished rewrite of Area.parse

Day10.lean
@@ -35,6 +35,9 @@ inductive Tile
 | start : Tile
 deriving BEq
 
+instance : Inhabited Tile where
+  default := Tile.ground
+
 -- The invariants are maybe overdoing it a bit, but (in the voice of king Leonidas) "This is Lean4!"
 structure Area where
   width : Nat
@@ -43,7 +46,6 @@ structure Area where
   fields : Array Tile
   size_invariant : fields.size = width * height
   start_invariant : fields[start.toIndex] = Tile.start
-  start_invariant2 : ∀ (index : Fin (width*height)), (index ≠ start.toIndex) → fields[index] ≠ Tile.start
 
 inductive Area.ParseError
 | NoInput
@@ -55,53 +57,35 @@ inductive Area.ParseError
 private structure Area.Raw where
   width : Nat
   height : Nat
-  start : Nat
+  start : Option $ Fin (width * height)
   fields : Array Tile
 
-private def Area.ParseRaw (input : String) : Except Area.ParseError Area.Raw := do
-  let lines := input.splitTrim (· == '\n')
-  -- Treat the first line special. We use it to establish width
-  match lines with
-  | [] => throw Area.ParseError.NoInput
-  | l :: ls =>
-    let mut width := 0
-    let mut arr : Array Tile := Array.empty
-    let mut start : Option Nat := none
-    for c in l.toSubstring do
-      let tile ← parse_character c |> Option.toExcept Area.ParseError.UnexpectedCharacter
-      arr := arr.push tile
-      if tile == Tile.start then
-        if start.isNone then
-          start := some width
-        else
-          throw Area.ParseError.MoreThanOneStart
-      width := width + 1
-    let mut height := 1
-    for line in ls do
-      let mut thisWidth := 0
-      for c in line.toSubstring do
-        let tile ← parse_character c |> Option.toExcept Area.ParseError.UnexpectedCharacter
-        arr := arr.push tile
-        if tile == Tile.start then
-          if start.isNone then
-            start := some (thisWidth * height)
-          else
-            throw Area.ParseError.MoreThanOneStart
-        thisWidth := thisWidth +1
-      height := height + 1
-      if thisWidth != width then
-        throw Area.ParseError.NotRectangular
-    if let some s := start then
-      return {
-        width := width,
-        height := height,
-        start := s,
-        fields := arr
-      }
+
+private def Area.parseLine (previous : Area.Raw) (pos : Nat) (line : Substring) (hh : previous.height > 0) : Except Area.ParseError (Nat × Area.Raw) :=
+  if h : line.isEmpty then
+    Except.ok (pos, previous)
+  else if h₀ : pos ≥ previous.width then
+    throw Area.ParseError.NotRectangular
+  else do
+    let tile ← Option.toExcept Area.ParseError.UnexpectedCharacter $ parseCharacter line.front
+    let rest := line.drop 1
+    if tile == Tile.start then
+      if previous.start.isSome then
+        throw Area.ParseError.MoreThanOneStart
+      else
+        have : previous.width * (previous.height - 1) + pos < previous.width * previous.height := by
+          have := Nat.mul_pred previous.width previous.height
+          simp only [Nat.pred_eq_sub_one] at this
+          rw[this]
+          have : previous.width ≤ previous.width*previous.height := Nat.le_mul_of_pos_right _ hh
+          rw[←Nat.sub_add_comm this]
+          omega
+        let start := ⟨previous.width * (previous.height - 1) + pos, this⟩
+        Area.parseLine {previous with fields := previous.fields.push tile, start := some start} (pos + 1) rest hh
     else
-      throw Area.ParseError.NoStart
-where
-  parse_character : Char → Option Tile := λ c ↦ match c with
+      Area.parseLine {previous with fields := previous.fields.push tile} (pos + 1) rest hh
+termination_by previous.width - pos
+where parseCharacter : Char → Option Tile := λ c ↦ match c with
   | '|' => some $ Tile.pipe Pipe.NS
   | '-' => some $ Tile.pipe Pipe.WE
   | 'L' => some $ Tile.pipe Pipe.NE
@@ -111,3 +95,273 @@ where
   | 'S' => some Tile.start
   | '.' => some Tile.ground
   | _ => none
+
+private theorem Nat.mul_le_succ_right : ∀ (n m : Nat), n*m ≤ n*m.succ := by
+  intro n m
+  rw[Nat.mul_succ]
+  omega
+
+private def Area.parseLines (previous : Area.Raw) (input : List String) : Except Area.ParseError Area.Raw :=
+  match input with
+  | [] => pure previous
+  | l :: ls => do
+    let current := {
+      previous with
+      height := previous.height + 1
+      start := Fin.castLE (Nat.mul_le_succ_right _ _) <$> previous.start
+    }
+    let (parsed_width, parsed_line) ← Area.parseLine current 0 l.toSubstring (by simp only [gt_iff_lt, Nat.zero_lt_succ])
+    if parsed_width = previous.width then
+      Area.parseLines parsed_line ls
+    else
+      throw Area.ParseError.NotRectangular
+
+private def Area.parseRaw (input : String) : Except Area.ParseError Area.Raw :=
+  let lines := input.splitTrim (· == '\n')
+  if h₁ : lines.isEmpty then
+    throw Area.ParseError.NoInput
+  else
+    have : 0 < lines.length := by
+      cases hl : lines
+      case nil => exact absurd (List.isEmpty_nil) (hl.subst (motive := λx↦¬x.isEmpty = true) h₁)
+      case cons => exact Nat.succ_pos _
+    let width := lines[0].length
+    if width > 0 then
+      let initial : Area.Raw := {
+        width,
+        height := 0,
+        start := none,
+        fields := Array.empty
+      }
+      Area.parseLines initial lines
+    else
+      throw Area.ParseError.NoInput
+
+private def Except.get (e : Except ε α) (_ : e.isOk) : α :=
+  match e with
+  | .ok a => a
+
+private theorem Area.ParseLine_adds_returned_count (previous : Area.Raw) (pos : Nat) (line : Substring) (h₁ : previous.height > 0) : (h : (Area.parseLine previous pos line h₁).isOk) → (Except.get (Area.parseLine previous pos line h₁) h).2.fields.size = previous.fields.size + (Except.get (Area.parseLine previous pos line h₁) h).1 - pos := by
+  intros h₂
+  generalize h₃ : Day10.Area.parseLine previous pos line h₁ = r at *
+  unfold parseLine at h₃
+  simp at h₃
+  split at h₃
+  case isTrue =>
+    subst r
+    unfold Except.get
+    simp
+  case isFalse =>
+    split at h₃
+    case isTrue => rw[←h₃] at h₂; contradiction
+    case isFalse =>
+      unfold bind Monad.toBind Except.instMonad at h₃
+      simp at h₃
+      cases h₄ : (Day10.Area.parseLine.parseCharacter line.front)
+      <;> simp[h₄, Option.toExcept, Except.bind] at h₃
+      case none => rw[←h₃] at h₂; contradiction
+      case some =>
+        split at h₃
+        case h_1 => rw[←h₃] at h₂; contradiction
+        case h_2 d1 h₅ char₂ d2 char h₆ =>
+        simp[Except.pure] at h₆
+        subst char₂
+        clear d1 d2
+        split at h₃
+        case' isTrue =>
+          split at h₃
+          case isTrue.isTrue => rw[←h₃] at h₂; contradiction
+          have : previous.width * (previous.height - 1) + pos < previous.width * previous.height := by
+            have := Nat.mul_pred previous.width previous.height
+            simp only [Nat.pred_eq_sub_one] at this
+            rw[this]
+            have : previous.width ≤ previous.width*previous.height := Nat.le_mul_of_pos_right _ h₁
+            rw[←Nat.sub_add_comm this]
+            omega
+          generalize hc :{ width := previous.width, height := previous.height, start := some ⟨previous.width * (previous.height - 1) + pos, this⟩, fields := previous.fields.push char : Area.Raw} = c
+        case' isFalse =>
+          generalize hc :{ width := previous.width, height := previous.height, start := previous.start, fields := previous.fields.push char : Area.Raw} = c
+        case isTrue | isFalse =>
+          simp[hc] at h₃
+          have : c.height = previous.height := by rw[←hc]
+          have h₆ := Area.ParseLine_adds_returned_count c (pos+1) (line.drop 1) (this▸h₁) (by simp_all)
+          simp[h₃] at h₆
+          have h₇ : c.fields.size = previous.fields.size + 1 := by
+            rw[←hc]
+            simp
+          rw[h₇] at h₆
+          omega
+termination_by previous.width - pos
+
+private theorem Area.ParseLine_leaves_width_and_height (previous : Area.Raw) (pos : Nat) (line : Substring) (h₁ : previous.height > 0) : (h : (Area.parseLine previous pos line h₁).isOk) → (Except.get (Area.parseLine previous pos line h₁) h).2.width = previous.width ∧ (Except.get (Area.parseLine previous pos line h₁) h).2.height = previous.height := by
+  intros h₂
+  generalize h₃ : Day10.Area.parseLine previous pos line h₁ = r at *
+  unfold parseLine at h₃
+  simp at h₃
+  split at h₃
+  case isTrue =>
+    subst r
+    unfold Except.get
+    simp
+  case isFalse =>
+    split at h₃
+    case isTrue => rw[←h₃] at h₂; contradiction
+    case isFalse =>
+      unfold bind Monad.toBind Except.instMonad at h₃
+      simp at h₃
+      cases h₄ : (Day10.Area.parseLine.parseCharacter line.front)
+      <;> simp[h₄, Option.toExcept, Except.bind] at h₃
+      case none => rw[←h₃] at h₂; contradiction
+      case some =>
+        split at h₃
+        case h_1 => rw[←h₃] at h₂; contradiction
+        case h_2 d1 h₅ char₂ d2 char h₆ =>
+        simp[Except.pure] at h₆
+        subst char₂
+        clear d1 d2
+        split at h₃
+        case' isTrue =>
+          split at h₃
+          case isTrue.isTrue => rw[←h₃] at h₂; contradiction
+          have : previous.width * (previous.height - 1) + pos < previous.width * previous.height := by
+            have := Nat.mul_pred previous.width previous.height
+            simp only [Nat.pred_eq_sub_one] at this
+            rw[this]
+            have : previous.width ≤ previous.width*previous.height := Nat.le_mul_of_pos_right _ h₁
+            rw[←Nat.sub_add_comm this]
+            omega
+          generalize hc :{ width := previous.width, height := previous.height, start := some ⟨previous.width * (previous.height - 1) + pos, this⟩, fields := previous.fields.push char : Area.Raw} = c
+        case' isFalse =>
+          generalize hc :{ width := previous.width, height := previous.height, start := previous.start, fields := previous.fields.push char : Area.Raw} = c
+        case isTrue | isFalse =>
+          simp[hc] at h₃
+          have h₇ : c.height = previous.height := by rw[←hc]
+          have h₆ := Area.ParseLine_leaves_width_and_height c (pos+1) (line.drop 1) (h₇▸h₁) (by simp_all)
+          simp[h₃] at h₆
+          have h₈ : c.width = previous.width := by rw[←hc]
+          omega
+termination_by previous.width - pos
+
+private theorem Area.ParseLines_array_size (input : Area.Raw) (lines : List String) (h₁ : input.fields.size = input.width * input.height) : (h : (Area.parseLines input lines).isOk) → (Except.get (Area.parseLines input lines) h).fields.size = (Except.get (Area.parseLines input lines) h).width * (Except.get (Area.parseLines input lines) h).height := by
+  intro h₂
+  generalize h₃ : Day10.Area.parseLines input lines = r at *
+  unfold Area.parseLines at h₃
+  cases lines <;> simp at h₃
+  case nil =>
+    simp[←h₃]
+    exact h₁
+  case cons l ls =>
+    unfold bind Monad.toBind Except.instMonad at h₃
+    simp at h₃
+    unfold Except.bind at h₃
+    split at h₃
+    case h_1 => rw[←h₃] at h₂; contradiction
+    case h_2 d lineResult h₄ =>
+      clear d
+      simp at h₃
+      split at h₃
+      case isFalse => rw[←h₃] at h₂; contradiction
+      case isTrue h₅ =>
+        simp[←h₃]
+        apply Area.ParseLines_array_size
+        have : (Area.parseLine { width := input.width, height := input.height + 1, start := Option.map (Fin.castLE (Nat.mul_le_succ_right _ _)) input.start, fields := input.fields } 0 l.toSubstring (Nat.succ_pos _)).isOk := by
+          cases hx : (Area.parseLine { width := input.width, height := input.height + 1, start := Option.map (Fin.castLE (Nat.mul_le_succ_right _ _)) input.start, fields := input.fields } 0 l.toSubstring (Nat.succ_pos _))
+          case error => rw[hx] at h₄; contradiction
+          case ok => rfl
+        have h₆ : lineResult.snd.width = input.width := by
+          have := Area.ParseLine_leaves_width_and_height { width := input.width, height := input.height + 1, start := Option.map (Fin.castLE (Nat.mul_le_succ_right _ _)) input.start, fields := input.fields } 0 l.toSubstring (Nat.succ_pos _) this
+          simp[Except.get] at this
+          split at this
+          rename_i lineResult₂ _ h₄₂ _
+          simp[h₄] at h₄₂
+          subst lineResult₂
+          exact this.left
+        have h₇ : lineResult.snd.height = input.height + 1 := by
+          have := Area.ParseLine_leaves_width_and_height { width := input.width, height := input.height + 1, start := Option.map (Fin.castLE (Nat.mul_le_succ_right _ _)) input.start, fields := input.fields } 0 l.toSubstring (Nat.succ_pos _) this
+          simp[Except.get] at this
+          split at this
+          rename_i lineResult₂ _ h₄₂ _
+          simp[h₄] at h₄₂
+          subst lineResult₂
+          exact this.right
+        have h₈ : lineResult.snd.fields.size = input.fields.size + lineResult.fst := by
+          have := Area.ParseLine_adds_returned_count { width := input.width, height := input.height + 1, start := Option.map (Fin.castLE (Nat.mul_le_succ_right _ _)) input.start, fields := input.fields } 0 l.toSubstring (Nat.succ_pos _) this
+          simp[Except.get] at this
+          split at this
+          rename_i lineResult₂ _ h₄₂ _
+          simp[h₄] at h₄₂
+          subst lineResult₂
+          assumption
+        rw[h₈, h₇, h₆, h₁, h₅]
+        exact Nat.mul_succ _ _
+
+
+private theorem Area.ParseRaw_array_size :
+  ∀ (input : String), (h : (Area.parseRaw input).isOk) → (Except.get (Area.parseRaw input) h).fields.size = (Except.get (Area.parseRaw input) h).width * (Except.get (Area.parseRaw input) h).height := by
+  intros input h₁
+  generalize h₂ : Day10.Area.parseRaw input = r at *
+  unfold Area.parseRaw at h₂
+  simp at h₂
+  split at h₂
+  case isTrue => rw[←h₂] at h₁; contradiction
+  split at h₂
+  case isFalse.isFalse => rw[←h₂] at h₁; contradiction
+  case isFalse.isTrue =>
+    simp[←h₂]
+    apply Area.ParseLines_array_size
+    rfl
+
+private theorem Except.isOk_exists {e : Except ε α} : (e.isOk = true) ↔ ∃a, e = Except.ok a := by
+  constructor
+  <;> intro h₁
+  case mp =>
+    match e with
+    | .ok v => exists v
+  case mpr =>
+    cases h₁
+    subst e
+    rfl
+
+private theorem Except.get_unfold {α : Type u1} {ε : Type u2} (v : α) : Except.get (α := α) (ε := ε) (Except.ok v) (rfl) = v := rfl
+
+private theorem Except.get_unfold' {α : Type u1} {ε : Type u2} {e : Except ε α} {v : α} (h₁ : e = Except.ok v) (h₂ : e.isOk) : Except.get e h₂ = v := by
+  simp[h₁]
+  apply Except.get_unfold
+
+private theorem Option.get_unfold {α : Type u} {v : α} : (some v).get (rfl) = v := rfl
+
+private theorem Option.get_unfold' {α : Type u} {o : Option α} {v : α} (h₁ : o = some v) (h₂ : o.isSome) : o.get h₂ = v := by
+  simp[h₁]
+
+private theorem Area.ParseRaw_start_position_aux :
+  ∀ (input : String), (h₁ : (Area.parseRaw input).isOk) →
+  match (Except.get (Area.parseRaw input) h₁).start with
+  | .some index => (Except.get (Area.parseRaw input) h₁).fields[index]! = Tile.start
+  | .none => True
+  := by
+  intros input h₁
+  split
+  case h_2 => trivial
+  case h_1 =>
+    generalize Day10.Area.parseRaw input = r at *
+    sorry
+
+private theorem Array.getElem!_eq_getElem {α : Type u} [Inhabited α] {a : Array α} {index : Nat} (h : index < a.size ): a[index] = a[index]! := by
+  unfold getElem getElem! instGetElem?OfGetElemOfDecidable Array.instGetElemNatLtSize decidableGetElem?
+  simp
+  split
+  <;> rename_i blah
+  <;> simp[h] at blah
+  assumption
+
+private theorem Area.ParseRaw_start_position :
+  ∀ (input : String), (h₁ : (Area.parseRaw input).isOk) → (h₂ : (Except.get (Area.parseRaw input) h₁).start.isSome) → (Except.get (Area.parseRaw input) h₁).fields[(Except.get (Area.parseRaw input) h₁).start.get h₂]'((Area.ParseRaw_array_size input h₁).substr ((Except.get (Area.parseRaw input) h₁).start.get h₂).isLt) = Tile.start := by
+  intros input h₁ h₂
+  have := Area.ParseRaw_start_position_aux input h₁
+  split at this
+  case h_2 hx => exact absurd h₂ (Option.not_isSome_iff_eq_none.mpr hx)
+  case h_1 maybeIndex index he =>
+    simp at this
+    simp_all
+    rw[←this]
+    apply Array.getElem!_eq_getElem
